\documentclass{gadsescript}
\usepackage{marvosym}

\settitle{Blatt 01}
\setsubtitle{Elias Gestrich}

\begin{document}
\maketitle
\section*{Aufgabe 1: Vektoren und Skalare}
\begin{enumerate}[label=\alph*)]
	\item ~
		\begin{enumerate}[label=\roman*)]
			\item $\vec a \cdot ( \vec b + \vec c) = \vec a \cdot \begin{pmatrix}3-7\\0+6\\-1+7\end{pmatrix} = \vec a \cdot \begin{pmatrix} -4\\6\\6\end{pmatrix} = -9 \cdot -4 + 0 \cdot 6 + 3 \cdot 6 = 54 $\\
			\item $ \vec a \mid \vec b + \vec c \mid = \vec a
				\mid\begin{pmatrix}-4\\6\\6\end{pmatrix}\mid 
				= \vec a \sqrt{(-4)^2 + 6^2 + 6^2} = \sqrt{16 + 36 + 36} \vec a = \sqrt{88} \, \vec a $
			\item $ \vec b \times ( \vec a \cdot \vec c ) = \vec b \times ( -7 \cdot -9 + 0 + 3 \cdot 7 ) = \vec b \times 84 $ \Lightning
			\item $ \vec b \cdot \vec c $ ist ein Skalar, ein Vektorprodukt ist nur f√ºr zwei Vektoren definiert \Lightning
			\item $ (\vec a \times \vec a) \cdot \vec c = \begin{pmatrix}0\\0\\0\end{pmatrix} \cdot \vec c = 0 $
			\item $ \vec c \times ( \vec b \times \vec a ) = \vec c \times
				\begin{pmatrix}
					0 \cdot 3 &- &-1 \cdot 0\\
					-(3 \cdot 3 &- &-1 \cdot -9)\\
					3 \cdot 0 &- &0 \cdot -9\\
				\end{pmatrix}
				= \vec c \times
				\begin{pmatrix}
					0\\
					0\\
					0
				\end{pmatrix}
				= \begin{pmatrix}0\\0\\0\end{pmatrix}
				$
		\end{enumerate}
	\item $\vec a \vec b = ab \cos(\vartheta) \iff \cos(\vartheta) = \frac{\vec a \vec b}{ab} = \frac{-27-3}{\sqrt{84}\sqrt{10}} = -\frac{30}{\sqrt{840}} \implies \vartheta = \arccos(\frac{30}{\sqrt{840}})$\\
		$\vec b \vec c = bc \cos(\vartheta) \iff \cos(\vartheta) = \frac{\vec b \vec c}{bc} = \frac{-21-7}{\sqrt{10}\sqrt{134}} = -\frac{28}{\sqrt{1340}} \implies \vartheta = \arccos(\frac{28}{\sqrt{1340}})$
	\item \begin{align*}
			\vec k \cdot \vec r &= \cos(\omega t)\exp(-\lambda t) \cdot \cos(\omega t) + \sin(\omega t) \exp(-\lambda t) \cdot \sin{\omega t} + \left( z - \frac{1}{2}\exp(-\lambda t) \right) \cdot 2\\
			~&= \exp(-\lambda t) \left( \cos^2(\omega t) + \sin^2(\omega t) + 1\right) + 2z\\
			~&= \exp(-\lambda t) (0) + 2z\\
			~&= 2z
	\end{align*}

\end{enumerate}

\end{document}
